src/resource_proofs.v
@@ -77,7 +77,7 @@ Definition as_tree (l : lmap M RI) : Branch M :=
   
 Definition lmap_is_borrow (lt: Lifetime) (loc: Loc RI) (m: M) (l : lmap M RI) :=
   forall pl , pl ∈ pls_of_loc loc ->
-    ∀ y , node_view (refinement_of_index M RI) (node_of_pl (as_tree l) pl) lt y -> tpcm_le m y.
+    ∀ y , node_view (refinement_of_nat M RI) (node_of_pl (as_tree l) pl) lt y -> tpcm_le m y.
 
 Definition is_borrow (lt: Lifetime) (loc: Loc RI) (m: M) (state: State M RI) :=
     match state with
@@ -88,7 +88,7 @@ Definition state_inv (state: State M RI) : Prop :=
   match state with
   | StateCon active l =>
        multiset_no_dupes active /\
-       branch_all_total_in_refinement_domain (refinement_of_index M RI) (as_tree l) active 0
+       branch_all_total_in_refinement_domain (refinement_of_nat M RI) (as_tree l) active 0
   end.
 
 Instance state_valid : Valid (State M RI) :=
@@ -190,12 +190,14 @@ Instance cell_op_proper_left :
 Instance cell_op_proper_right n :
     Proper ((≡) ==> (≡)) (cell_op n). Admitted.
 
-
 Instance node_view_proper roi :
     Proper ((≡) ==> (=) ==> (=) ==> impl) (node_view roi). Admitted.
     
 Instance node_live_proper :
     Proper ((≡) ==> (=)) node_live. Admitted.
+
+Instance node_total_minus_live_proper ref:
+    Proper ((≡) ==> (=) ==> (=)) (node_total_minus_live ref). Admitted.
     
 Instance cell_live_proper :
     Proper ((≡) ==> (=)) cell_live. Admitted.
@@ -225,12 +227,15 @@ Lemma exists_some_of_match {A} (t: option A) (is_some : match t with | Some _ =>
 (*node_view roi (a ⋅ b) k -> node_view roi a k
             (node_of_pl (build gamma (CellCon m ∅) ⋅ as_tree l2 ⋅ as_tree l0)
                (any_pl_of_loc gamma)) kappa
-            (node_total_minus_live (refinement_of_index M RI)
+            (node_total_minus_live (refinement_of_nat M RI)
                (node_of_pl (build gamma (CellCon m ∅) ⋅ as_tree l2 ⋅ as_tree l0)
                   (any_pl_of_loc gamma))
                (multiset_add (multiset_add (multiset_add kappa empty_lifetime) l1) l))*)
 
 Lemma node_view_le roi a b lt y : node_view roi (a ⋅ b) lt y -> node_view roi a lt y.
+Admitted.
+
+Lemma node_view_le2 roi a lt y z : node_view roi a lt y -> node_view roi a lt (dot y z).
 Admitted.
 
 Lemma node_view_strip roi a b c loc kappa x :
@@ -305,12 +310,6 @@ Proof.
   trivial.
 Qed.
 
-(****************************************************************)
-(****************************************************************)
-(****************************************************************)
-(****************************************************************)
-(* borrow(kappa, gamma, z) . live(gamma, m) . live(alpha ref gamma, y)
-                         --> live(gamma, m') . live(alpha ref gamma, y') *)
 
 Definition borrow_exchange_cond (ref: Refinement M M) (z m f m' f' : M) :=
   ∀ p , match rel M M ref (dot (dot f z) p) with
@@ -324,9 +323,9 @@ Definition borrow_exchange_cond (ref: Refinement M M) (z m f m' f' : M) :=
   
 Lemma multiset_add_empty (a : Lifetime) :
   multiset_add a empty_lifetime = a. Admitted.
-  
-Definition view_exchange_cond (ref: Refinement M M) (view: M -> Prop) (m f m' f' : M) :=
-  ∀ p , view p -> match rel M M ref (dot f p) with
+    
+Definition specific_exchange_cond (ref: Refinement M M) (p m f m' f' : M) :=
+  match rel M M ref (dot f p) with
   | None => True
   | Some i1 => m_valid (dot m i1) ->
       match rel M M ref (dot f' p) with
@@ -335,23 +334,91 @@ Definition view_exchange_cond (ref: Refinement M M) (view: M -> Prop) (m f m' f'
       end
   end.
   
-Definition flow_cond p i (b t t': Branch M) (active: Lifetime) (down up : PathLoc -> M) :=
+Definition view_exchange_cond (ref: Refinement M M) (view: M -> Prop) (m f m' f' : M) :=
+  ∀ p , view p -> specific_exchange_cond ref p m f m' f'.
+  
+Definition specific_flow_cond p i (t t': Branch M) (active: Lifetime) (down up : PathLoc -> M) :=
   let q := (p, i) in
   let r := (p, S i) in
   let s := (p ++ [i], 0) in
-  view_exchange_cond (refinement_of_index M RI i)
-      (node_view (refinement_of_index M RI) (node_of_pl b q) active)
+  specific_exchange_cond (refinement_of_nat M RI i)
+      (node_total_minus_live (refinement_of_nat M RI) (node_of_pl t q) active)
       (dot (down q) (up r))
       (dot (up s) (node_live (node_of_pl t q)))
       (dot (up q) (down r))
       (dot (down s) (node_live (node_of_pl t' q))).
+  
+Definition view_flow_cond p i (b t t': Branch M) (active: Lifetime) (down up : PathLoc -> M) :=
+  let q := (p, i) in
+  let r := (p, S i) in
+  let s := (p ++ [i], 0) in
+  view_exchange_cond (refinement_of_nat M RI i)
+      (node_view (refinement_of_nat M RI) (node_of_pl b q) active)
+      (dot (down q) (up r))
+      (dot (up s) (node_live (node_of_pl t q)))
+      (dot (up q) (down r))
+      (dot (down s) (node_live (node_of_pl t' q))).
+      
+Lemma specific_flows_preserve_branch_all_total_in_refinement_domain t t' active
+  (down up : PathLoc -> M)
+  (flow_update : ∀ p i , specific_flow_cond p i t t' active down up)
+  (batird : branch_all_total_in_refinement_domain (refinement_of_nat M RI) t active 0)
+          : branch_all_total_in_refinement_domain (refinement_of_nat M RI) t' active 0.
+Admitted.
+
+Lemma multiset_le_refl `{EqDecision A, Countable A} (x: multiset A)
+  : multiset_le x x. Admitted.
+
+Lemma specific_exchange_cond_add_stuff (ref: Refinement M M) (p m f m' f' stuff : M) :
+  specific_exchange_cond ref (dot p stuff) m f m' f' -> specific_exchange_cond ref p m (dot f stuff) m' (dot f' stuff).
+Proof. unfold specific_exchange_cond. intro. rewrite <- tpcm_assoc.
+rewrite <- tpcm_assoc. assert (dot p stuff = dot stuff p) by (apply tpcm_comm).
+rewrite <- H0. trivial. Qed.
+
+Lemma node_live_op (n1 n2 : Node M) : node_live (n1 ⋅ n2) = dot (node_live n1) (node_live n2).
+Admitted.
 
 Lemma flows_preserve_branch_all_total_in_refinement_domain b t t' active
   (down up : PathLoc -> M)
-  (flow_update : ∀ p i , flow_cond p i b t t' active down up)
-  (batird : branch_all_total_in_refinement_domain (refinement_of_index M RI) (t⋅b) active 0)
-          : branch_all_total_in_refinement_domain (refinement_of_index M RI) (t'⋅b) active 0.
-Admitted.
+  (flow_update : ∀ p i , view_flow_cond p i b t t' active down up)
+  (batird : branch_all_total_in_refinement_domain (refinement_of_nat M RI) (t⋅b) active 0)
+          : branch_all_total_in_refinement_domain (refinement_of_nat M RI) (t'⋅b) active 0.
+Proof.
+  apply specific_flows_preserve_branch_all_total_in_refinement_domain with
+      (t := t⋅b) (down := down) (up := up); trivial.
+  intros.
+  unfold specific_flow_cond. unfold view_flow_cond in flow_update.
+  have flow_update' := flow_update p i. clear flow_update. rename flow_update' into flow_update.
+  unfold view_exchange_cond in flow_update.
+  
+  assert (node_live (node_of_pl (t ⋅ b) (p, i)) =
+      dot (node_live (node_of_pl t (p, i))) (node_live (node_of_pl b (p,i))))
+  by (setoid_rewrite <- forall_node_op; apply node_live_op).
+  rewrite H. clear H.
+  
+  assert (node_live (node_of_pl (t' ⋅ b) (p, i)) =
+      dot (node_live (node_of_pl t' (p, i))) (node_live (node_of_pl b (p,i))))
+  by (setoid_rewrite <- forall_node_op; apply node_live_op).
+  rewrite H. clear H.
+  
+  rewrite tpcm_assoc. rewrite tpcm_assoc.
+  
+  apply specific_exchange_cond_add_stuff.
+  
+  apply flow_update. clear flow_update.
+  apply node_view_le2.
+  apply node_view_le with (b := node_of_pl t (p, i)).
+  setoid_rewrite node_op_comm.
+  setoid_rewrite forall_node_op.
+  
+  assert (view_sat (node_view (refinement_of_nat M RI) (node_of_pl (t ⋅ b) (p, i)) active)
+    (node_total_minus_live (refinement_of_nat M RI) (node_of_pl (t ⋅ b) (p, i)) active)).
+  - apply node_view_le_total_minus_live with (idx := plend (p,i)).
+    * apply multiset_le_refl.
+    * generalize batird. rewrite forall_equiv_branch_all_total_in_refinement_domain.
+        intro. apply H.
+  - unfold view_sat in H. trivial.
+Qed.
 
 Lemma assoc_comm (a b c : Branch M) : (a ⋅ b) ⋅ c ≡ (a ⋅ c) ⋅ b.
 Proof.
@@ -413,26 +480,34 @@ Lemma updog_other_eq_unit p i alpha ri gamma m
   (is_not_in : (p, i) ∉ pls_of_loc gamma)
     : (updog m gamma alpha ri (p ++ [i], 0)) = unit. Admitted.
     
+Lemma specific_exchange_cond_of_no_change ref p x y
+  : specific_exchange_cond ref p x y x y. Admitted.
+    
 Lemma view_exchange_cond_of_no_change ref view x y
   : view_exchange_cond ref view x y x y.
 Proof. unfold view_exchange_cond. intro.
   assert (exists t , t = rel M M ref (dot y p)) by (exists (rel M M ref (dot y p)); trivial).
-  deex.
+  deex. unfold specific_exchange_cond.
   rewrite <- H. destruct t; crush.
   apply reflex.  
 Qed.
 
 Lemma unit_dot_left a : dot unit a = a. Admitted.
 
-Definition node_live_op (n1 n2: Node M) : node_live (n1 ⋅ n2) = dot (node_live n1) (node_live n2). Admitted.
-
 Lemma pl_not_in_of_pl_in_extloc pl alpha (ri: RI) gamma
   : pl ∈ pls_of_loc (ExtLoc alpha ri gamma) -> pl ∉ pls_of_loc gamma. Admitted.
   
-Lemma refinement_of_index_eq_refinement_of_of_in_pls_of_loc p i alpha ri gamma
+Lemma refinement_of_nat_eq_refinement_of_of_in_pls_of_loc p i alpha ri gamma
   (is_in : (p, i) ∈ pls_of_loc (ExtLoc alpha ri gamma))
-    : refinement_of_index M RI i = refinement_of ri.
+    : refinement_of_nat M RI i = refinement_of ri.
     Admitted.
+    
+(****************************************************************)
+(****************************************************************)
+(****************************************************************)
+(****************************************************************)
+(* borrow(kappa, gamma, z) . live(gamma, m) . live(alpha ref gamma, y)
+                         --> live(gamma, m') . live(alpha ref gamma, y') *)
   
 Lemma view_exchange_cond_of_borrow_exchange_cond alpha ri gamma z m f m' f' p i borrow_branch
   (i_matches : (p, i) ∈ pls_of_loc (ExtLoc alpha ri gamma))
@@ -440,13 +515,13 @@ Lemma view_exchange_cond_of_borrow_exchange_cond alpha ri gamma z m f m' f' p i 
   (exchange_cond : borrow_exchange_cond (refinement_of ri) z m f m' f')
   (isb : lmap_is_borrow active_lifetime (ExtLoc alpha ri gamma) z borrow_branch)
   : view_exchange_cond
-    (refinement_of_index M RI i)
-    (node_view (refinement_of_index M RI) (node_of_pl (as_tree borrow_branch) (p,i)) active_lifetime)
+    (refinement_of_nat M RI i)
+    (node_view (refinement_of_nat M RI) (node_of_pl (as_tree borrow_branch) (p,i)) active_lifetime)
     m f m' f'.
 Proof.
-  have h := refinement_of_index_eq_refinement_of_of_in_pls_of_loc p i alpha ri gamma.
+  have h := refinement_of_nat_eq_refinement_of_of_in_pls_of_loc p i alpha ri gamma.
   rewrite h; trivial. clear h.
-  unfold view_exchange_cond. unfold borrow_exchange_cond in *.
+  unfold view_exchange_cond. unfold specific_exchange_cond. unfold borrow_exchange_cond in *.
   unfold lmap_is_borrow in *.
   intro extra. intro.
   assert (tpcm_le z extra).
@@ -489,7 +564,7 @@ Proof.
       (down := updog m gamma alpha ri)
       (up   := updog m' gamma alpha ri); trivial.
     
-    intros. unfold flow_cond.
+    intros. unfold view_flow_cond.
     have the_case : Decision ((p, i) ∈ pls_of_loc (ExtLoc alpha ri gamma)) by solve_decision.
     destruct the_case.
     
@@ -556,4 +631,159 @@ Proof.
         rewrite build_rest_triv; trivial.
         rewrite tpcm_comm.
         apply view_exchange_cond_of_no_change.
+Qed.
+
+(****************************************************************)
+(****************************************************************)
+(****************************************************************)
+(****************************************************************)
+(* live(I(f), gamma) -> live(f, alpha ref gamma) *)
+
+Definition is_fresh_nat : Branch M -> nat -> Prop. Admitted.
+
+Definition alloc_alpha : Branch M -> RI -> nat. Admitted.
+
+Lemma is_fresh_alloc branch ri : is_fresh_nat branch
+    (nat_of_extstep (alloc_alpha branch ri) ri). Admitted.
+
+Lemma trivial_node_at_fresh (b: Branch M) p i
+  (is_fresh: is_fresh_nat b i)
+  : node_trivial (node_of_pl b (p, i)). Admitted.
+
+Tactic Notation "full_generalize" constr(t) "as" simple_intropattern(name) :=
+  let EQ := fresh in
+  let name1 := fresh in
+  assert (exists x , x = t) as EQ by (exists t; trivial); destruct EQ as [name1];
+    rewrite <- EQ;
+    (repeat match reverse goal with  
+    | [H : context[t] |- _ ] => rewrite <- EQ in H
+    end); clear EQ; try (clear name); rename name1 into name.
+    
+Lemma i_value_of_pls_of_loc_ext p i gamma alpha (ri: RI)
+  (in_pls: (p, i) ∈ pls_of_loc (ExtLoc alpha ri gamma))
+  : i = nat_of_extstep alpha ri. Admitted.
+
+Lemma node_total_minus_live_of_trivial ref node lt
+  (istriv: node_trivial node)
+  : node_total_minus_live ref node lt = unit. Admitted.
+
+Lemma cell_triv_node_triv_op_right a b
+  (nodetriv: node_trivial (a ⋅ b))
+  : cell_trivial (match b with CellNode c _ => c end). Admitted.
+
+Lemma ri_of_nat_nat_of_extstep alpha ri
+  : ri_of_nat RI (nat_of_extstep alpha ri) = ri. Admitted.
+
+Lemma initialize_ext gamma m f p ri
+  (is_rel: rel M M (refinement_of ri) f = Some m)
+  (si: state_inv (live gamma m ⋅ p))
+  : ∃ alpha , state_inv (live (ExtLoc alpha ri gamma) f ⋅ p).
+Proof.
+  destruct p. unfold live in si. rename l0 into p.
+  exists (alloc_alpha (build gamma (CellCon m ∅) ⋅ as_tree p) ri).
+  unfold state_inv, live, "⋅", state_op in *. destruct_ands. split; trivial.
+  
+  rename H0 into batird.
+  setoid_rewrite <- as_tree_dot.
+  setoid_rewrite <- as_tree_dot in batird.
+  
+  setoid_rewrite as_tree_singleton.
+  setoid_rewrite as_tree_singleton in batird.
+  
+  full_generalize (multiset_add empty_lifetime l) as lt.
+  full_generalize (as_tree p) as q. clear p.
+  
+  apply specific_flows_preserve_branch_all_total_in_refinement_domain
+    with (t := (build gamma (CellCon m ∅) ⋅ q))
+         (down := updog m gamma (alloc_alpha (branch_op (build gamma (CellCon m ∅)) q) ri) ri)
+         (up   := λ pl, unit); trivial.
+  intros. 
+  
+  assert (is_fresh_nat (branch_op (build gamma (CellCon m ∅)) q) (nat_of_extstep (alloc_alpha (branch_op (build gamma (CellCon m ∅)) q) ri) ri)) by (apply is_fresh_alloc; trivial).
+  rename H0 into is_fresh.
+  
+  full_generalize (alloc_alpha (branch_op (build gamma (CellCon m ∅)) q) ri) as alpha.
+  
+  
+  unfold specific_flow_cond.
+  repeat (rewrite unit_dot_left).
+  repeat (rewrite unit_dot).
+   
+  intros.
+  have the_case : Decision ((p, i) ∈ pls_of_loc (ExtLoc alpha ri gamma)) by solve_decision.
+  destruct the_case.
+
+  (* interesting case: ext location *)
+  
+  - rewrite (updog_eq_m p i); trivial. 
+    rewrite (updog_eq_unit1 p i); trivial.
+    rewrite (updog_eq_unit2 p i); trivial.
+    rewrite <- forall_node_op. rewrite <- forall_node_op.
+    repeat (rewrite unit_dot).
+    repeat (rewrite unit_dot_left).
+    rewrite node_live_op. rewrite node_live_op.
+    rewrite node_node_cell_cell. rewrite node_node_cell_cell.
+    rewrite node_node_cell_cell.
+    
+    assert ((p, i) ∉ pls_of_loc gamma) by (apply pl_not_in_of_pl_in_extloc with (alpha:=alpha) (ri:=ri); trivial ).
+    rewrite build_rest_triv; trivial.
+    
+    rewrite build_spec; trivial.
+    unfold cell_live, triv_cell.
+    
+    assert (node_trivial (node_of_pl ((build gamma (CellCon m ∅)) ⋅ q) (p, i))) as EqTrivNode by (
+      apply trivial_node_at_fresh;
+      rewrite <- (i_value_of_pls_of_loc_ext p i gamma) in is_fresh; trivial).
+    
+    rewrite <- forall_node_op in EqTrivNode.
+    
+    rewrite node_total_minus_live_of_trivial; trivial.
+    
+    have h := (cell_triv_node_triv_op_right _ _ EqTrivNode).
+    unfold cell_of_pl. destruct (node_of_pl q (p, i)).
+    unfold cell_trivial in h. destruct c. destruct_ands.
+    subst m0.
+    
+    unfold specific_exchange_cond.
+    repeat (rewrite unit_dot). unfold refinement_of_nat.
+    have j := i_value_of_pls_of_loc_ext p i gamma alpha ri e. rewrite j.
+    rewrite ri_of_nat_nat_of_extstep.
+    rewrite is_rel.
+    rewrite rel_unit.
+    repeat (rewrite unit_dot).
+    repeat (rewrite unit_dot_left).
+    intro. apply reflex.
+    
+    - have the_case2 : Decision ((p, i) ∈ pls_of_loc gamma) by solve_decision.
+      destruct the_case2.
+      
+      (* semi-interesting case: base location *)
+      + 
+        rewrite <- (updog_other_eq_both p i); trivial.
+        rewrite (updog_base_eq_m p i); trivial.
+        
+        rewrite <- forall_node_op. rewrite <- forall_node_op.
+        rewrite node_live_op. rewrite node_live_op.
+        repeat (rewrite unit_dot).
+        rewrite node_node_cell_cell. rewrite node_node_cell_cell.
+        rewrite node_node_cell_cell.
+        rewrite build_spec; trivial.
+        rewrite build_rest_triv; trivial.
+        unfold cell_live, triv_cell.
+        repeat (rewrite unit_dot_left).
+        apply specific_exchange_cond_of_no_change.
+
+      (* uninteresting case *)
+      + 
+        rewrite <- (updog_other_eq_both p i); trivial.
+        rewrite updog_other_eq_unit; trivial.
+
+        rewrite <- forall_node_op. rewrite <- forall_node_op.
+        rewrite node_live_op. rewrite node_live_op.
+        rewrite node_node_cell_cell. rewrite node_node_cell_cell.
+        rewrite node_node_cell_cell.
+        rewrite build_rest_triv; trivial.
+        rewrite build_rest_triv; trivial.
+        repeat (rewrite unit_dot_left).
+        apply specific_exchange_cond_of_no_change.
 Qed.
